src/QuerySemantic.v
@@ -27,12 +27,17 @@ Section QuerySemantic.
 
   Variables N Name Vals : ordType.
   
- 
   
+  Ltac case_response r := case: r => [l | l v | l vs | l ρ | l ρs].
+    
   Section Aux.    
     Variables (T1 T2 : Type).
     
-   
+    Equations indexed_map_In s (f : forall (i : nat) (x : T1), In x s -> T2) (index : nat) : seq T2 :=
+      { 
+        indexed_map_In [::] _ _ := [::];
+        indexed_map_In (hd :: tl) f i := (f i hd _) :: (indexed_map_In tl (fun i x H => f i x _) i.+1)
+      }.
       
     (**
        indexed_map : (s : seq T1) -> (nat -> x : T1 -> x ∈ s -> T2) -> seq T2
@@ -43,15 +48,31 @@ Section QuerySemantic.
        applied belongs to the list. This is mainly to be able to prove some
        obligations afterwards.
      **)
-    Equations indexed_map (s : list T1) (f : forall (i : nat) (x : T1), In x s -> T2)  : list T2 :=
-       indexed_map s f := indexed_map_In s f 0
+    Definition indexed_map (s : list T1) (f : forall (i : nat) (x : T1), In x s -> T2)  : list T2 :=
+        indexed_map_In s f 0
+    .
     
-    where indexed_map_In s (f : forall (i : nat) (x : T1), In x s -> T2) (index : nat) : seq T2 :=
-            { 
-              indexed_map_In [::] _ _ := [::];
-              indexed_map_In (hd :: tl) f i := (f i hd _) :: (indexed_map_In tl (fun i x H => f i x _) i.+1)
-            }.
+
+    Lemma indexed_map_In_n (s : list T1) (f : T1 -> T2) :
+      forall n1 n2,
+        indexed_map_In s (fun _ x _ => f x) n1 = indexed_map_In s (fun _ x _ => f x) n2.
+    Proof.
+      elim: s => //= hd tl IH n1 n2; simp indexed_map_In.
+      congr cons.
+      apply: IH.
+    Qed.
     
+    Lemma indexed_map_eq_map (s : list T1) (f : T1 -> T2) :
+      indexed_map s (fun _ x _ => f x) = [seq f x | x <- s].
+    Proof.
+      elim: s => //= hd tl IH.
+      rewrite /indexed_map; simp indexed_map_In.
+      congr cons.
+      rewrite -IH /=.
+      rewrite /indexed_map.
+      apply: indexed_map_In_n.
+    Qed.
+      
     Variables (T : Type) (dflt : T).
 
 
@@ -110,6 +131,8 @@ Section QuerySemantic.
     
   End Aux.
 
+  Arguments indexed_map_In [T1 T2].
+  Arguments indexed_map [T1 T2].
   Arguments indexed_map  [T1 T2].
   Arguments get_nth [T].
   
@@ -127,20 +150,22 @@ Section QuerySemantic.
          an empty list is returned, which gets deleted when the flattening occurs.
        **)
       
-      Equations indexed_β_filter (responses : seq.seq (@ResponseObject Name Vals)) (filter :  @ResponseObject Name Vals) (index : nat) : seq.seq (@ResponseObject Name Vals) :=
+      Equations indexed_β_filter (filter :  @ResponseObject Name Vals) (responses : seq (@ResponseObject Name Vals))  (index : nat) : seq.seq (@ResponseObject Name Vals) :=
         {
-          indexed_β_filter [::] _ _ := [::];
-          indexed_β_filter (cons hd tl) filter index :=
-            (β_aux hd filter index) ++ (indexed_β_filter tl filter index)
-            where β_aux (result flt : @ResponseObject Name Vals) (i : nat) : seq.seq (@ResponseObject Name Vals) :=
-                    {
-                      β_aux (NestedListResult l rs) (NestedListResult l' rs') i with l == l' :=
-                        {
-                        | true := get_nth [::] rs i;
-                        | false => [::]
-                        };
-                      β_aux _ _ _ := [::]
-                    }
+          indexed_β_filter _ [::] _ := [::];
+          indexed_β_filter filter (hd :: tl) index :=
+            (β_aux filter hd index) ++ (indexed_β_filter filter tl index)
+            where
+            β_aux (flt result : @ResponseObject Name Vals) (i : nat) : seq (@ResponseObject Name Vals) :=
+              {
+                β_aux (NestedListResult l' _) (NestedListResult l rs)  i
+                  with l == l' :=
+                  {
+                  | true := get_nth [::] rs i;
+                  | false => [::]
+                  };
+                β_aux _ _ _ := [::]
+              }
         }.
     
     
@@ -150,13 +175,14 @@ Section QuerySemantic.
     
   
       Lemma indexed_β_size_reduced (lst : seq.seq ResponseObject) (r : ResponseObject) (i : nat) :
-        responses_size (indexed_β_filter lst r i) <= responses_size lst.
+        responses_size (indexed_β_filter r lst i) <= responses_size lst.
       Proof.
-        apply (@indexed_β_filter_elim (fun rsp flt index res => responses_size res <= responses_size rsp)
-                                      (fun hd tl flt index r1 r2 i res => responses_size res <= response_size r1)) => //.
-        - move=> hd tl flt index IH IH'.
-          rewrite responses_size_app /=. ssromega.
-        -  move=> l1 l2 hd tl flt index rs rs' i'.
+        apply (indexed_β_filter_elim
+                 (fun flt rsp index res => responses_size res <= responses_size rsp)
+                 (fun flt hd tl index r1 r2 i res => responses_size res <= response_size r2)) => //.
+        - move=> flt hd tl index IH IH'.
+          by rewrite responses_size_app /=; ssromega.
+        -  move=> l1 l2 flt hd tl index rs' rs i'.
           
           funelim (get_nth [::] rs i') => //= Heq.
           simp response_size. ssromega.
@@ -164,9 +190,27 @@ Section QuerySemantic.
           rewrite [responses_size t + _]addnC. 
           rewrite two_times_Sn; rewrite [4 + (2 * size l + 2)]addnA.
           rewrite -addnA -[2 + _]addnCA addnA; rewrite -[4 + 2 * size l + responses_size' l]/(response_size (NestedListResult l1 l)).
-            by move: (H lst r i l1 l2 hd tl flt index rs' Heq ) => *; apply: leq_addr. 
+            by move: (H lst r i l1 l2 flt hd tl index rs' Heq ) => *; apply: leq_addr. 
       Qed.
-          
+      
+      Lemma indexed_β_nil :
+        forall flt rs i,
+        all (fun r => ~~partial_response_eq flt r) rs ->
+        indexed_β_filter flt rs i = [::].
+      Proof.
+        apply (indexed_β_filter_elim
+                 (fun flt rsp index res =>
+                    all (fun r => ~~partial_response_eq flt r) rsp ->
+                    res = [::])
+                 (fun flt hd tl index r1 r2 i res =>
+                    ~~partial_response_eq r1 r2 ->
+                    res = [::])) => //=.
+        - move=> flt hd tl i IH IH' /andP [Hhd Htl].
+            by rewrite IH // IH'.
+
+        - by move=> l l' _ _ _ _ _ l2 i /eqP -> /eqP.
+      Qed.
+
       
     End Indexed_Beta.
 
@@ -216,7 +260,21 @@ Section QuerySemantic.
         rewrite responses_size_app.
         by simp response_size; ssromega.
       Qed.
-  
+
+      Lemma β_filter_nil flt rs :
+        all (fun r => ~~partial_response_eq flt r) rs ->
+        β_filter flt rs = [::].
+
+      Proof.
+        elim: rs => //= hd tl IH /andP [Hhd Htl].
+        case: flt IH Hhd Htl => //.
+        move=> f rs IH Hhd Htl; simp β_filter.
+        rewrite {}IH // cats0.
+        case: hd Hhd => // {Htl} f' rs'; simp β.
+        rewrite /partial_response_eq => /eqP.
+        by case: eqP => //= ->.
+      Qed.
+      
     End Beta.
 
         Section Gamma.
@@ -236,15 +294,7 @@ Section QuerySemantic.
           γ _ _ => false
         }.
 
-      Definition partial_response_eq (r1 r2 : @ResponseObject Name Vals) : bool :=
-        match r1, r2 with
-        | (SingleResult l v), (SingleResult l' v') => (l == l') && (v == v')
-        | (ListResult l v), (ListResult l' v') => (l == l') && (v == v')
-        | (Null l), (Null l') => l == l'
-        | (NestedResult l _), (NestedResult l' _) => l == l' 
-        | (NestedListResult l _), (NestedListResult l' _) => l == l'   
-        | _, _ => false
-        end.
+
       (**
          γ_filter : ResponseObject -> seq ResponseObject -> seq ResponseObject 
          Filters out response objects that are partially equal to the filter
@@ -262,8 +312,8 @@ Section QuerySemantic.
           }
         }.*)
 
-      Definition γ_filter (flt : @ResponseObject Name Vals) (responses : seq.seq (@ResponseObject Name Vals)) : seq.seq (@ResponseObject Name Vals) :=
-        filter (fun r => ~~partial_response_eq flt r) responses.
+      Definition γ_filter (flt : @ResponseObject Name Vals) (responses : seq (@ResponseObject Name Vals)) : seq (@ResponseObject Name Vals) :=
+        [seq r <- responses | ~~partial_response_eq flt r].
       
 
 
@@ -279,8 +329,23 @@ Section QuerySemantic.
         case: ifP => // H.
         simpl. ssromega.
         ssromega.
-        Qed.
-        
+      Qed.
+
+      Lemma γ_filter_same_with_no_eq flt rs :
+        all (fun r => ~~partial_response_eq flt r) rs ->
+        γ_filter flt rs = rs.
+      Proof.
+        elim: rs => //= hd tl IH /andP [Hhd Htl].
+        rewrite Hhd.
+        by rewrite IH.
+      Qed.
+
+      Lemma γ_filter_cat flt s1 s2 :
+        γ_filter flt (s1 ++ s2) = γ_filter flt s1 ++ γ_filter flt s2.
+      Proof.
+        by rewrite /γ_filter filter_cat. 
+      Qed.
+      
     End Gamma.
     
   End Filters.
@@ -306,7 +371,7 @@ Section QuerySemantic.
                          (NestedListResult l
                            (indexed_map rs             
                               (fun i r (H : In r rs) =>
-                                 (collect (r ++ (indexed_β_filter tl (NestedListResult l rs) i))))))
+                                 (collect (r ++ (indexed_β_filter (NestedListResult l rs) tl i))))))
                            :: (collect (γ_filter (NestedListResult l rs) tl));
                                
       collect (cons hd tl) := hd :: (collect (γ_filter hd tl)).
@@ -337,71 +402,212 @@ Section QuerySemantic.
   Next Obligation.
       by move: (γ_responses_size_reduced tl (NestedListResult l rs)) => *; simp response_size; ssromega.
   Qed.
+
+
+
+  Lemma collect_nr_with_no_eq l ρ tl :
+    all (fun r => ~~partial_response_eq (NestedResult l ρ) r) tl ->
+    collect (NestedResult l ρ :: tl) = (NestedResult l (collect ρ)) :: collect tl.
+  Proof.
+    move=> Hneq; simp collect.
+    rewrite β_filter_nil //=; rewrite cats0.
+    rewrite γ_filter_same_with_no_eq //.
+  Qed.
+
+
+  Lemma indexed_map_In_eq l :
+    forall ρ n tl χ,
+      all (fun r => ~~partial_response_eq (NestedListResult l χ) r) tl ->
+    indexed_map_In ρ
+    (fun (i : nat) (r : seq ResponseObject) (_ : In r ρ) => collect (r ++ indexed_β_filter (NestedListResult l χ) tl i)) n =
+    indexed_map_In ρ (fun (_ : nat) (r : seq ResponseObject) (_ : In r ρ) => collect r) n.
+  Proof.
+    elim=> // hd tl IH n tl0 χ Hneq; simp indexed_map_In.
+    rewrite indexed_β_nil // cats0.
+    congr cons.
+    apply (IH n.+1 tl0 χ Hneq).
+  Qed.
+  
+  
+  Lemma collect_nlr_with_no_eq l ρ tl :
+    all (fun r => ~~partial_response_eq (NestedListResult l ρ) r) tl ->
+    collect (NestedListResult l ρ :: tl) = (NestedListResult l (indexed_map ρ (fun i r H => collect r))) :: collect tl.
+  Proof.
+    move=> Hneq; simp collect.
+    rewrite γ_filter_same_with_no_eq //.
+    congr cons; congr NestedListResult.
+    rewrite /indexed_map.
+    by apply indexed_map_In_eq.
+  Qed.
+
+  
+  Lemma filter_preserves_non_redundancy flt responses :
+    are_non_redundant__ρ responses ->
+    are_non_redundant__ρ (γ_filter flt responses).
+  Proof.
+    elim: responses => //= hd tl IH.
+    case Hhas: has => //=.
+    move/andP=> [Hnr Hnrtl].
+    case: ifP => //; last first.
+      by move=> _; apply: IH => //=.
+    rewrite are_non_redundant__ρ_equation_2.
+    case Hhas': has => //=.  
+    move/negbT: Hhas => /hasPn Hhas.
+    move/hasP: Hhas' => [q].
+    rewrite mem_filter => /andP [Hneq Hin].
+    by move: (Hhas q Hin) => /negbTE ->.
+    by move=> _; apply/andP; split => //; apply IH.
+  Qed.
+
+  
+    
+  Lemma γ_filter_eq flt s :
+    has (fun r => partial_response_eq flt r) s = false ->
+    γ_filter flt s = s.
+  Proof.
+    elim: s => // hd tl IH /hasPn H /=.
+    case: ifP => // Heq.
+    rewrite IH //.
+    apply/hasPn => x Hin.
+      by apply: H; apply: mem_tail.
+    have Hin : hd \in hd :: tl by apply: mem_head.
+      by move: (H hd Hin); rewrite Heq.
+  Qed.
+
+  
+  Lemma β_filter_eq flt s :
+    has (fun r => partial_response_eq flt r) s = false ->
+    β_filter flt s = [::].
+  Proof.
+    elim: s => // hd tl IH /hasPn.
+    case: hd => // [l | l v | l vs | l ρ | l ρs] Hhas; simp β_filter; case: flt IH Hhas => //.
+    all: do ?[by intros; simp β; rewrite cat0s IH //;
+              apply/hasPn => x Hin; apply: Hhas; apply: mem_tail].
+
+    move=> l' χ IH Hhas; simp β.
+    case: eqP => //= Heq.
+    - move: (Hhas (NestedResult l ρ) (mem_head (NestedResult l ρ) _)) => /= /eqP.
+      by rewrite Heq.
+    - apply: IH; apply/hasPn=> x Hin.
+      by apply: Hhas; apply: mem_tail.
+  Qed.
+
+  Lemma indexed_β_eq flt s i :
+     has (fun r => partial_response_eq flt r) s = false ->
+     indexed_β_filter flt s i = [::].
+  Proof.
+    elim: s => // hd tl IH /hasPn.
+    case: hd => // [l | l v | l vs | l ρ | l ρs] Hhas; simp indexed_β_filter => /=; case: flt IH Hhas => //.
+
+    all: do ?[by intros=> /=; apply: IH; apply/hasPn => x Hin; apply: Hhas; apply: mem_tail].
+
+    move=> l' χ IH Hhas /=.
+    case: eqP => Heq //=.
+    move: (Hhas (NestedListResult l ρs) (mem_head (NestedListResult l ρs) _)) => /= /eqP.
+      by rewrite Heq.
+    by apply: IH; apply/hasPn => x Hin; apply: Hhas; apply: mem_tail.
+  Qed.
+
+
+ (* Lemma indexed_map_In_eq_2 s s2 flt:
+    are_non_redundant__ρ s2 ->
+    (forall (i : nat) (r : seq ResponseObject),
+       In r s ->
+       are_non_redundant__ρ (r ++ indexed_β_filter flt s2 i) ->
+       collect (r ++ indexed_β_filter flt s2 i) = r ++ indexed_β_filter flt s2 i) ->
+    all (fun x : response_eqType Name Vals => ~~ partial_response_eq flt x) s2 ->
+    (indexed_map s
+       (fun (i : nat) (r : seq ResponseObject) (_ : In r s) => collect (r ++ indexed_β_filter flt s2 i))) =
+    s.
+  Proof.
+    elim: s s2 => // hd tl IH s2 Hnr H Hall.
+    rewrite /indexed_map; simp indexed_map_In.
+  *)
+
+  Lemma map_collect_eq flt s1 s2 i :
+    has (partial_response_eq flt) s2 = false ->
+    all (are_non_redundant__ρ (Vals:=Vals)) s1 ->
+    (forall r : seq ResponseObject,
+        In r s1 ->
+        are_non_redundant__ρ (r ++ indexed_β_filter flt s2 i) ->
+        collect (r ++ indexed_β_filter flt s2 i) = r ++ indexed_β_filter flt s2 i) ->
+    [seq collect x | x <- s1] = s1.
+  Proof.
+    move=> Hhas.
+    rewrite indexed_β_eq //.
+    move=> Hnr H.
+    elim: s1 Hnr H => //= hd tl IH /andP [Hnr Hnrs] H.
+    have/(H hd): hd = hd \/ In hd tl by left.
+    rewrite cats0; move/(_ Hnr) => ->; congr cons.
+    apply: IH => //.
+    by move=> r Hin Hnr'; apply: H => //; right.
+  Qed.
+  
+  Lemma collect_non_redundant_eq ρ :
+    are_non_redundant__ρ ρ ->
+    collect ρ = ρ.
+  Proof.
+    
+    apply_funelim (collect ρ) => //= [l | l v | l vs | l χ | l ρs] tl IH.
+   
+    all: do ?[by case Hhas : has => //= /andP [Hnr Hnrs]; do ?[congr cons]; rewrite γ_filter_eq // in IH *; apply: IH].
+  
+    - move=> IH'.
+      case Hhas: has => //= /andP.
+      simp is_non_redundant__ρ; case=> [Hnr Hnrs]. 
+      rewrite β_filter_eq // ?cats0 ?γ_filter_eq // in IH IH' *.
+      by rewrite IH // IH'.
+
+    - rewrite -collect_equation_6.
+      
+      move=> IH'.
+      case Hhas: has => //= /andP.
+      simp is_non_redundant__ρ; case=> [Hnr Hnrs].
+      rewrite collect_nlr_with_no_eq // ?indexed_map_eq_map.
+      rewrite ?γ_filter_eq // in IH IH' *; rewrite IH' //.
+      congr cons; congr NestedListResult.
+      pose i := 0.
+      move: (IH i) => H.
+      apply: (map_collect_eq (NestedListResult l ρs) ρs tl i) => //.
+      by move/hasPn: Hhas => /allP.
+  Qed.
+
+  Lemma collect_preserves_non_redundancy ρs :
+    are_non_redundant__ρ ρs ->
+    are_non_redundant__ρ (collect ρs).
+  Proof.
+      by move=> Hnr; rewrite collect_non_redundant_eq.
+  Qed.
+    
+    
+  Lemma in_collect_γ r flt ρ :
+    r \in collect (γ_filter flt ρ) ->
+    ~~partial_response_eq flt r.
+  Proof.
+    elim: ρ flt => //= hd tl IH flt.
+    case: ifP => Heq; last by apply: IH.
+    case: hd Heq => //= [l | l v | l vs | l ρ | l ρs] Heq; simp collect; rewrite inE => /orP [/eqP -> // | Hin];
+    apply: IH.
+    
+  Admitted.
+  
+  Lemma collect_are_non_redundant ρs :
+    are_non_redundant__ρ (collect ρs).
+  Proof.
+    elim: ρs => // hd tl IH.
+  Admitted.
+    
+    
+    
+ 
+
+
   
   Implicit Type schema : @wfSchema Name Vals.
   Implicit Type graph : @graphQLGraph Name Vals.
   Implicit Type u : @node Name Vals.
   Implicit Type query : @Query Name Vals.
 
-  (*
-  Fixpoint eval schema graph u query : seq.seq ResponseObject :=
-    match query with
-    | SingleField name args => match u.(fields) (Field name args) with
-                              | Some (inl value) =>  [:: SingleResult name value]
-                              | _ => [:: Null name]
-                              end
-    | LabeledField label name args =>  match u.(fields) (Field name args) with
-                                      | Some (inl value) => [:: SingleResult label value]
-                                      | _ => [:: Null label]
-                                      end
-    | NestedField name args ϕ => let target_nodes := get_target_nodes_with_field graph u (Field name args) in
-                                match lookup_field_type schema u.(type) name with
-                                | Some (ListType _) =>
-                                  [:: NestedListResult name [seq (eval_queries schema graph v ϕ) | v <- target_nodes]]
-                                    
-                                | Some (NT _) =>
-                                  match ohead target_nodes with
-                                  | Some v => [:: NestedResult name (eval_queries schema graph v ϕ)]
-                                  | _ =>  [:: Null name]
-                                  end
-                                | _ => [:: Null name]         (* If the field ∉ fields(u) then it's null, right? *)
-                                end
-                                    
-    | NestedLabeledField label name args ϕ =>  let target_nodes := get_target_nodes_with_field graph u (Field name args) in
-                                              match lookup_field_type schema u.(type) name with
-                                              | Some (ListType _) =>
-                                                [:: NestedListResult label [seq (eval_queries schema graph v ϕ) | v <- target_nodes]]
-                                              | Some (NT _) =>
-                                                match ohead target_nodes with
-                                                | Some v => [:: NestedResult label (eval_queries schema graph v ϕ)]
-                                                | _ => [:: Null label]
-                                                end
-                                              | _ => [:: Null label]
-                                              end
-    | InlineFragment t ϕ => match lookup_type schema t with
-                           | Some (ObjectTypeDefinition _ _ _) => if t == u.(type) then
-                                                                   (eval_queries schema graph u ϕ)
-                                                                 else
-                                                                   [::]
-                           | Some (InterfaceTypeDefinition _ _) => if declares_implementation schema u.(type) t then
-                                                                   (eval_queries schema graph u ϕ)
-                                                                  else
-                                                                    [::]
-                           | Some (UnionTypeDefinition _ mbs) => if u.(type) \in mbs then
-                                                                   (eval_queries schema graph u ϕ)
-                                                                else
-                                                                  [::]
-                           | _ =>  [::]
-                           end
-    end
-  with
-  eval_queries schema graph u (queries : seq (@Query Name Vals)) {struct queries} : seq (@ResponseObject Name Vals) :=
-    match queries with
-    | [::] => [::]
-    | query :: [::] => eval schema graph u query
-    | query :: (hd :: tl) => collect ((eval schema graph u query) ++ (eval schema graph u hd) ++ (eval_queries schema graph u tl))
-    end.
-   *)
   
   Equations eval schema graph u query : seq.seq (@ResponseObject Name Vals) :=
     {
@@ -449,64 +655,59 @@ Section QuerySemantic.
         end;
       
       eval schema graph u (InlineFragment t ϕ)
-        with [|| (is_object_type schema t && (u.(type) == t)),
-              u.(type) \in implementation schema t |
-              u.(type) \in union_members schema t] :=
+        with u.(type) == t :=
         {
-        | true := eval_queries schema graph u ϕ;
-          | _ := [::]
+        | true  := eval_queries schema graph u ϕ;
+        | _ with u.(type) \in implementation schema t :=
+            {
+            | true := eval_queries schema graph u ϕ;
+            | _ with u.(type) \in union_members schema t :=
+                {
+                | true := eval_queries schema graph u ϕ;
+                | _ := [::]
+                }
+            }
         }
     }
   where
   eval_queries schema graph u (queries : seq (@Query Name Vals)) : seq (@ResponseObject Name Vals) :=
     {
       eval_queries _ _ _ [::] := [::];
-      eval_queries schema graph u (cons query nil) := eval schema graph u query;
-      eval_queries schema graph u (cons query (cons hd tl)) := collect ((eval schema graph u query) ++ (eval schema graph u hd) ++ (eval_queries schema graph u tl))
+      eval_queries schema graph u (query :: tl) :=  collect ((eval schema graph u query) ++ (eval_queries schema graph u tl))
     }.
 
-  (*
-  Definition eval_queries schema graph u (queries : seq.seq Query) : seq.seq ResponseObject :=
-    collect (flatten (map (eval schema graph u) queries)).
-   *)
 
-  (*
-  Lemma eval_single_field schema graph u f α :
-    (exists v, eval schema graph u (SingleField f α) = [:: SingleResult f v]) \/
-    eval schema graph u (SingleField f α) = [:: Null f].
+  Lemma eval_non_redundant :
+    forall schema g u φ,
+    are_non_redundant__ρ (eval schema g u φ).
   Proof.
-    rewrite eval_equation_1.
-    case Hv : (u.(fields) (Field f α)) => [val|]; last by right.
-    case: val Hv => val Hv.
-      by left; exists val.
-      by right.
+    apply (eval_elim
+             (fun schema g u q res =>
+                are_non_redundant__ρ res)
+             (fun schema g u qs res =>
+                are_non_redundant__ρ res)) => //=.
+    - intros. case Hlook: lookup_field_type => [rty|] //.
+      case: rty Hlook => //= ty Hlook.
+      case: ohead => [fld|] //=; rewrite andbT; simp is_non_redundant__ρ; apply: H => //; exact: (NT ty).
+      rewrite andbT; simp is_non_redundant__ρ.
+      apply/allP => x /mapP [r Hin ->]; apply: H; exact: ty.
+
+     - intros. case Hlook: lookup_field_type => [rty|] //.
+      case: rty Hlook => //= ty Hlook.
+      case: ohead => [fld|] //=; rewrite andbT; simp is_non_redundant__ρ; apply: H => //; exact: (NT ty).
+      rewrite andbT; simp is_non_redundant__ρ.
+      apply/allP => x /mapP [r Hin ->]; apply: H; exact: ty.
+
+     - intros.
+       apply: collect_are_non_redundant.
   Qed.
 
-    Lemma eval_labeled_field schema graph u l f α :
-    (exists v, eval schema graph u (LabeledField l f α) = [:: SingleResult l v]) \/
-    eval schema graph u (LabeledField l f α) = [:: Null l].
+  Lemma eval_queries_are_non_redundant schema g u φ :
+    are_non_redundant__ρ (eval_queries schema g u φ).
   Proof.
-    rewrite eval_equation_2.
-    case Hv : (u.(fields) (Field f α)) => [val|]; last by right.
-    case: val Hv => val Hv.
-      by left; exists val.
-      by right.
+      by case: φ => //= hd tl; apply: collect_are_non_redundant.
   Qed.
-  
-
-  Lemma eval_single_field_size_1 schema graph u f α :
-    size (eval schema graph u (SingleField f α)) = 1.
-  Proof.
-    move: (eval_single_field schema graph u f α) => [| ->] //.
-      by case=> v ->.
-  Qed. *)
-
-  Lemma collect_app_nil r :
-    collect (r ++ [::]) = collect r.
-  Proof.
-      by rewrite cats0.
-  Qed.
-
+      
   Lemma gamma_filter_single_result_null f f' v (lst : seq (@ResponseObject Name Vals)) :
     γ_filter (SingleResult f v) ((Null f') :: lst) = (Null f') :: γ_filter (SingleResult f v) lst. Proof. done. Qed.
 
@@ -520,42 +721,190 @@ Section QuerySemantic.
   Proof. done. Qed.
 
 
- (* Lemma collect_nested_result l r :
-    collect [:: NestedResult l r] = [:: NestedResult l (collect r)].
+  Lemma γ_filter_swap flt1 flt2 s :
+    γ_filter flt1 (γ_filter flt2 s) = γ_filter flt2 (γ_filter flt1 s).
   Proof.
-    funelim (collect [:: NestedResult l r]) => //=.
-      by rewrite collect_equation_1 collect_app_nil.
-  Qed. *)
+    elim: s => //= hd tl IH.
+    case: ifP => Hpeq /=;
+    case: ifP => Hpeq2 /=.
 
-  Lemma collect_nested_list_result (l : Name) (r : seq (seq (@ResponseObject Name Vals))) :
-    collect [:: NestedListResult l r] = [:: NestedListResult l (map collect r)].
+    all: do ?[by rewrite Hpeq IH].
+    all: do ?[by rewrite IH].
+  Qed.
+  
+  Lemma collect_γ_filter flt lst :
+    γ_filter flt (collect (γ_filter flt lst)) = collect (γ_filter flt lst).
   Proof.
   Admitted.
-  
 
-  
 
-  
+  Hint Resolve collect_are_non_redundant.
   Lemma collect_collect_same (r : seq (@ResponseObject Name Vals)) :
     collect r = collect (collect r).
   Proof.
-  Admitted.
+    rewrite [collect (collect r)]collect_non_redundant_eq //.
+  Qed.
 
+  Hint Resolve eval_non_redundant eval_queries_are_non_redundant.
+  Lemma eval_collect_same :
+    forall schema graph u query,
+      eval schema graph u query = collect (eval schema graph u query).
+  Proof.
+    intros; rewrite collect_non_redundant_eq //.
+  Qed.
+   (* apply (eval_elim
+             (fun schema g u q res =>
+                res = collect res)
+             (fun schema g u qs res =>
+                res = collect res)) => schema g u.
+    - move=> f α φ /= IH1 IH2.
+      case Hty: lookup_field_type => [rty|] //=.
+      case: rty Hty => // rty Hty.
+      case: ohead => [v|] //=.
+      rewrite collect_nr_with_no_eq //=; simp collect.
+      rewrite -IH1 //; exact: (NT rty).
+      rewrite collect_nlr_with_no_eq //=; simp collect.
+      congr cons; congr NestedListResult.
+      rewrite indexed_map_eq_map /=.
+      rewrite -map_comp /= /funcomp.
+
+      have H: (forall v : node, eval_queries schema g v φ = collect (eval_queries schema g v φ)) ->
+            forall s, [seq eval_queries schema g v φ | v <- s] =
+                 [seq collect (eval_queries schema g v φ) | v <- s].
+      move=> H; elim=> //= hd tl IH.
+        by rewrite -H IH.
+      apply: H.
+      by apply: IH2.  
+
+    - move=> l f α φ /= IH1 IH2.
+      case Hty: lookup_field_type => [rty|] //=.
+      case: rty Hty => // rty Hty.
+      case: ohead => [v|] //=.
+      rewrite collect_nr_with_no_eq //=; simp collect.
+      rewrite -IH1 //; exact: (NT rty).
+      rewrite collect_nlr_with_no_eq //=; simp collect.
+      congr cons; congr NestedListResult.
+      rewrite indexed_map_eq_map /=.
+      rewrite -map_comp /= /funcomp.
+
+      have H: (forall v : node, eval_queries schema g v φ = collect (eval_queries schema g v φ)) ->
+            forall s, [seq eval_queries schema g v φ | v <- s] =
+                 [seq collect (eval_queries schema g v φ) | v <- s].
+      move=> H; elim=> //= hd tl IH.
+        by rewrite -H IH.
+      apply: H.
+      by apply: IH2.  
+
+    all: do ?[by intros; simp collect].
+      
+    - move=> hd tl IHhd IHtl.
+      by rewrite -collect_collect_same.
+  Qed.*)
+
+
+  Lemma eval_queries_collect_same schema graph u qs :
+    eval_queries schema graph u qs = collect (eval_queries schema graph u qs).
+  Proof.
+    by rewrite collect_non_redundant_eq //. 
+  Qed.
+  
   Lemma eval_same_query_in_list schema graph u query :
     eval schema graph u query = eval_queries schema graph u [:: query].
-  Proof. done. Qed.
-
+  Proof.
+    rewrite eval_queries_equation_2 /= cats0.
+      by apply: eval_collect_same.
+  Qed.
+  
   Lemma eval_query_inline schema (g : conformedGraph schema) qs :
     eval schema g g.(root) (InlineFragment schema.(query_type) qs) = eval_queries schema g g.(root) qs.
   Proof.
     simp eval.
-    move: (query_has_object_type schema) => ->.
     move: (root_query_type  g) => -> /=.
     by case: eqP.
   Qed.
+
+  Lemma γ_collect_γ flt s :
+    γ_filter flt (collect (γ_filter flt s)) = collect (γ_filter flt s).
+  Proof.
+    elim: s => //= hd tl IH.
+    case: flt IH => [l | l v | l vs | l ρ | l ρs] IH; case: ifP => //.
+    Admitted.
+
+
+  
+  Lemma collect_collect_2_cat s1 s2 :
+    collect (collect s1 ++ s2) = collect (s1 ++ s2).
+  Proof.
+    elim: s1 s2 => // hd tl IH s2.
+    case_response hd; simp collect; do ? rewrite -/(cat _ _).
+    congr cons.
+    rewrite 2!γ_filter_cat γ_collect_γ.
     
+    (*
+    elim: s2 s1 => // [| hd tl IH] s1.
+    - by rewrite 2!cats0 -collect_collect_same.
+    - 
+      case: s1 => //= hd' tl'.
+      case: hd' => //.
+      move=> l; rewrite ?collect_equation_2 -/(cat _ _).
+      congr cons.
+      rewrite 2!γ_filter_cat.
+      
+
+  Abort. *)
+    
+      
+  Lemma collect_collect_3_cat s1 s2 s3 :
+    collect (collect(s1 ++ s2) ++ s3) =
+    collect (s1 ++ collect(s2 ++ s3)).
+  Proof.
+    elim: s1 s2 s3 => // [| hd tl IH] s2 s3.
+    rewrite 2!cat0s.
+    elim: s2 s3 => //=.
+    - by move=> s3; simp collect; rewrite cat0s -collect_collect_same.
+    - move=> hd tl IH s3.
+  Abort.
+
+  Lemma eval_collect_cat schema g u s1 s2 :
+    eval_queries schema g u (s1 ++ s2) =
+    collect (eval_queries schema g u s1 ++ eval_queries schema g u s2).
+  Proof.
+    elim: s2 s1 => // [ /=| hd tl IH] s1.
+    - by rewrite 2!cats0 -eval_queries_collect_same.
+
+    -
 
 
+      
+  Lemma collect_eval_cat schema g u s1 s2 :
+    collect (eval_queries schema g u s1 ++ eval_queries schema g u s2) =
+    eval_queries schema g u (s1 ++ s2).
+  Proof.
+    elim: s2 s1 => //=.
+    - intros; rewrite !cats0.
+        by rewrite -eval_queries_collect_same.
+
+    - move=> hd tl IH s1.
+      rewrite [RHS]eval_queries_collect_same.
+      
+    elim: s1 s2 => //=.
+    - move=> s2. by rewrite -eval_queries_collect_same.
+    - move=> hd tl IH s2.
+  Admitted.
+  
+  Lemma implementation_nil_for_object schema ty :
+    is_object_type schema ty ->
+    implementation schema ty = fset0.
+  Proof.
+    funelim (is_object_type schema ty) => //= _.
+    rewrite /implementation.
+  Admitted.
+
+  Lemma union_nil_for_object schema ty :
+    is_object_type schema ty ->
+    union_members schema ty = fset0.
+  Admitted.
+    
     
   Lemma inline_nested_empty schema (g : @conformedGraph Name Vals schema) :
     forall t1 t2 ϕ,
@@ -565,12 +914,13 @@ Section QuerySemantic.
       eval schema g g.(root) (InlineFragment t1 [:: (InlineFragment t2 ϕ)]) = [::].
   Proof.
     move=> t1 t2 ϕ Hobj Hobj' /eqP /negbTE Hneq /=.
-    simp eval; rewrite Hobj andTb.
-    case: or3P => //=. 
-    simp eval; rewrite Hobj'.
-    case: or3P => //=.
-  Admitted.
-
+    move: (query_has_object_type schema).
+    move: (root_query_type g) => <- Hscope.
+    simp eval.
+    case: eqP => //= Heq; [simp eval; rewrite Heq Hneq /=|];
+    rewrite implementation_nil_for_object //=;
+    rewrite union_nil_for_object //=.
+  Qed.
   
 
   Lemma inline_query_preserves schema (g : @conformedGraph Name Vals schema):
@@ -609,19 +959,22 @@ Section QuerySemantic.
   Proof.
     move=> Hqs.
     do 2 rewrite eval_equation_3.
-    case lookup_field_type => //.
+    case lookup_field_type => //=.
     case=> [nt | lt].
     case neighbours_with_field => // v1 vn /=.
-    case ohead => // node.
-      by move: (Hqs node) => ->. 
+      by rewrite Hqs.
     case neighbours_with_field => // v1 vn /=.
     congr cons.
     congr NestedListResult.
-    
+    rewrite Hqs.
+    congr cons.
   Admitted.
+
+  
     
+      
 End QuerySemantic.
 
-
+Arguments collect [Name Vals].
 Arguments eval [Name Vals].
 Arguments eval_queries [Name Vals].
