src/QueryEq.v
@@ -80,9 +80,29 @@ Section Eq.
     congr cons.
     by rewrite (H hd).
   Qed.
+
+
+  Lemma implementation_nil_for_union schema ty :
+    is_union_type schema ty ->
+    implementation schema ty = fset0.
+  Admitted.
+
+  Lemma collect_nested_cat (s1 s2 : seq (@ResponseObject Name Vals)) :
+    collect (collect s1 ++ collect s2) = collect (s1 ++ s2).
+  Admitted.
+  
+  Lemma eval_collect_cat schema graph u qs1 qs2 :
+    collect (eval_queries schema graph u qs1 ++ eval_queries schema graph u qs2) =
+    eval_queries schema graph u (qs1 ++ qs2).
+  Proof.
+    rewrite [RHS]eval_queries_collect_same.
+    congr collect.
+  Abort.
     
   Lemma normalize_preserves_eval :
     forall schema ty φ (g : @conformedGraph Name Vals schema) u,
+      u \in g.(nodes) ->
+      u.(type) \in get_possible_types schema ty ->
       query_conforms schema ty φ ->
       has_valid_fragments schema ty φ ->
       eval schema g u φ =  eval_queries schema g u (normalize schema ty φ).
@@ -90,57 +110,93 @@ Section Eq.
     apply (normalize_elim
              (fun schema ty q nqs =>
                 forall (g : @conformedGraph Name Vals schema) u,
+                  u \in g.(nodes) ->
+                  u.(type) \in get_possible_types schema ty ->
                   query_conforms schema ty q ->
                   has_valid_fragments schema ty q ->
                   eval schema g u q = eval_queries schema g u nqs)
              (fun schema ty qs nqs =>
                 forall (g : @conformedGraph Name Vals schema) u,
+                  u \in g.(nodes) ->
+                  u.(type) \in get_possible_types schema ty ->
                   all (query_conforms schema ty) qs ->
                   all (has_valid_fragments schema ty) qs ->
                   eval_queries schema g u qs = eval_queries schema g u nqs)) => schema //.
+    
 
-    - move=> ty f α Hscope g u Hqc Hv.
+    all: do ?[by intros; apply: eval_same_query_in_list].
+
+     
+    - move=> ty f α Hscope g u Hin Hupty Gqc Hv.
       simp try_inline_query.
       case: eqP => //= Hpty.
-      by apply: inlined_query_eq_eval.
-
-    - move=> ty l f α Hscope g u Hqc Hv.
+      * by rewrite cats0; apply: eval_collect_same.
+      * by apply: inlined_query_eq_eval.
+        
+     
+    - move=> ty l f α Hscope g u _ _ Hqc Hv.
       simp try_inline_query.
       case: eqP => //= Hpty.
-        by apply: inlined_query_eq_eval.
+      * by rewrite cats0; apply: eval_collect_same.
+      * by apply: inlined_query_eq_eval.
 
-    all: do ?[by intros; rewrite /query_conforms Heq in H].
+    all: do ?[by intros; rewrite /query_conforms Heq in H1].
 
-    - move=> ty f fld α φ IH Hscope Hlook g u Hqc Hv /=.
-      simp eval => /=.
-      move: Hqc; rewrite /query_conforms Hlook => /and4P [_ _ _ Hqsc].
-      move: Hv; simp has_valid_fragments; rewrite Hlook => Hv.
-      case: lookup_field_type => [rty|] //=.
-      case: rty => [nty | lty].
-      case: ohead => [v |] //=.
-        by rewrite IH.
-      congr cons.
-      congr (NestedListResult f).  
-      apply: map_normalize_eval_eq => v.
-        by apply: (IH g v).
+    
+    - admit.
+    - admit.
+    - admit.
+    - admit.
+      
+    - move=> t b ty φ IH Ht Hscope g u Hin.
+      rewrite get_possible_types_objectE //= inE => Huty /and4P [_ _ _ Hqsc].
+      simp has_valid_fragments; rewrite Hscope /= => /andP [/eqP Hteq Hv].
+      rewrite -Hteq in Huty.
+      simp eval; rewrite Huty /=.
+      apply: IH => //=.
+        by rewrite get_possible_types_objectE //= inE -Hteq.
+        by rewrite Hteq in Hqsc.
 
-    - move=> ty f fld α φ IH Hscope Hlook g u Hqc Hv /=.
-      simp try_inline_query.
-      case: eqP => //= Hpty.
-      simp eval => /=.
-      move: Hqc; rewrite /query_conforms Hlook => /and4P [_ _ _ Hqsc].
-      move: Hv; simp has_valid_fragments; rewrite Hlook => Hv.
-      case: lookup_field_type => [rty|] //=.
-      case: rty => [nty | lty].
-      case: ohead => [v |] //=.
-        by rewrite IH.
-      congr cons.
-      congr (NestedListResult f).  
-      apply: map_normalize_eval_eq => v.
-        by apply: (IH g v).
+    - move=> t ty φ IH Ht Hscope g u Hin Hpty Hqc Hv.
+      move: Hqc => /= /and4P [_ _ _] Hqc.
+      move: Hv; simp has_valid_fragments; rewrite Hscope /= => /andP [_] Hv.  
 
-        admit.
-        Admitted.
+ 
+      simp eval; case: eqP => Heq //=.
+      * rewrite cats0.
+        rewrite -IH //.
+          by apply: eval_queries_collect_same.
+          by rewrite get_possible_types_objectE //= inE Heq.
+          by rewrite implementation_nil_for_object //= union_nil_for_object.
+            
+    - move=> t ty φ IH Ht Hscope g u Hin Hpty Hqc Hv; simp eval.
+      case: eqP => //= Heq.
+      * move: (node_in_graph_has_object_type Hin) => Huty.
+        by rewrite Heq Ht in Huty.
+
+      * move: (type_in_scope_N_obj_is_abstract Hqc Hscope).
+        move: Hv; simp has_valid_fragments; rewrite Hscope /= => {Heq} /andP [/orP [/eqP Heq | Hcontr] Hv]; last first.
+          by rewrite Hcontr in Ht.
+        rewrite /is_abstract_type => /orP [Hintf | Hunion].
+        rewrite get_possible_types_interfaceE // in Hpty IH.
+        rewrite -Heq in Hpty IH *.
+        rewrite Hpty /=.
+        apply: IH => //.
+          by move: Hqc; rewrite /query_conforms => /and4P [_ _ _].
+
+        rewrite get_possible_types_unionE // in Hpty IH.
+        rewrite -Heq in Hpty IH Hunion *.
+
+        rewrite implementation_nil_for_union //= Hpty /=.
+        apply: IH => //.
+          by move: Hqc; rewrite /query_conforms => /and4P [_ _ _].
+
+    - move=> ty hd tl IHhd IHtl g u Hin Hpty.
+      all_cons => [Hqc Hqsc].
+      all_cons => [Hv Hvs] /=.
+      rewrite IHhd // IHtl //.
+        by apply: collect_eval_cat.
+  Qed.
         
 
   
@@ -156,16 +212,15 @@ Section Eq.
       all (has_valid_fragments schema ty) (normalize__φ schema ty qs).
   Admitted.
   
-  Lemma remove_redundancies_eval_eq schema (g : @conformedGraph Name Vals schema) u φ φs :
-    eval schema g u φ = eval_queries schema g u φs ->
-    eval schema g u φ = eval_queries schema g u (remove_redundancies φs).
+  Lemma remove_redundancies_eval_eq schema (g : @conformedGraph Name Vals schema) u φs :
+    eval_queries schema g u φs = eval_queries schema g u (remove_redundancies φs).
   Proof.
     apply_funelim (remove_redundancies φs) => //.
 
-    intros => /=.
-    case: γ__φ.
     Admitted.
-  
+
+ 
+
   Theorem all_q_has_nrgtnf_q schema (g : @conformedGraph Name Vals schema):
     forall (φ : @Query Name Vals) ty,
       query_conforms schema ty φ ->
@@ -177,7 +232,9 @@ Section Eq.
          all (has_valid_fragments schema ty) φ',
          are_in_normal_form schema φ',
          are_non_redundant φ' &
-         forall u, eval schema g u φ = eval_queries schema g u φ'].
+         forall u, u \in g.(nodes) ->
+              u.(type) \in get_possible_types schema ty ->
+                    eval schema g u φ = eval_queries schema g u φ'].
   Proof.
     case=> [f α | l f α | f α φ | l f α φ | t φ] ty Hqc Hv;
     [ exists [:: SingleField f α]
@@ -191,8 +248,59 @@ Section Eq.
     all: do ?[by apply: remove_redundancies_preserves_valid_fragments; apply: normalize_preserves_valid_fragments].
     all: do ?[by apply: remove_redundancies_normalize_preserves_normal_form].
     all: do ?[by apply: remove_redundancies_is_non_redundant].
-    all: do ?[by move=> u; apply: remove_redundancies_eval_eq; apply: normalize_preserves_eval].
+    all: do ?[by move=> u Hin Hty; rewrite -remove_redundancies_eval_eq; apply: normalize_preserves_eval].
   Qed.
       
-       
+
+   Theorem bleble schema (g : @conformedGraph Name Vals schema) :
+    forall (φ : @Query Name Vals),
+      query_conforms schema schema.(query_type) φ ->
+      has_valid_fragments schema schema.(query_type) φ ->
+
+      exists (φ' : seq Query),
+        [/\
+         all (query_conforms schema schema.(query_type)) φ',
+         all (has_valid_fragments schema schema.(query_type)) φ',
+         are_in_normal_form schema φ',
+         are_non_redundant φ' &
+         eval schema g g.(root) φ = eval_queries schema g g.(root) φ'].
+  Proof.
+    case=> [f α | l f α | f α φ | l f α φ | t φ] Hqc Hv;
+    [ exists [:: SingleField f α]
+    | exists [:: LabeledField l f α]
+    | exists (remove_redundancies (normalize schema schema.(query_type) (NestedField f α φ)))
+    | exists (remove_redundancies (normalize schema schema.(query_type) (NestedLabeledField l f α φ)))
+    | exists (remove_redundancies (normalize schema schema.(query_type) (InlineFragment t φ)))]; split=> //.
+
+    all: do ?[by rewrite all_seq1].
+    all: do ?[by apply: remove_redundancies_preserves_conformance; apply: normalize_preserves_conformance].
+    all: do ?[by apply: remove_redundancies_preserves_valid_fragments; apply: normalize_preserves_valid_fragments].
+    all: do ?[by apply: remove_redundancies_normalize_preserves_normal_form].
+    all: do ?[by apply: remove_redundancies_is_non_redundant].
+
+    rewrite -remove_redundancies_eval_eq.
+    apply: normalize_preserves_eval => //.
+    apply: root_in_nodes.
+    rewrite get_possible_types_objectE //=.
+    rewrite mem_seq1.
+    apply/eqP. apply: root_query_type.
+    apply: query_has_object_type.
+
+    rewrite -remove_redundancies_eval_eq.
+    apply: normalize_preserves_eval => //.
+    apply: root_in_nodes.
+    rewrite get_possible_types_objectE //=.
+    rewrite mem_seq1.
+    apply/eqP. apply: root_query_type.
+    apply: query_has_object_type.
+
+    rewrite -remove_redundancies_eval_eq.
+    apply: normalize_preserves_eval => //.
+    apply: root_in_nodes.
+    rewrite get_possible_types_objectE //=.
+    rewrite mem_seq1.
+    apply/eqP. apply: root_query_type.
+    apply: query_has_object_type.
+  Qed.
+  
 End Eq.
